scripts/hol-probes/regenerate.sh
@@ -218,6 +218,9 @@ run_probe crep_inline_code_inl_probeScript.sml crep_inline_code_inl_probe.out \
   "$cake_dir/pancake"
 run_probe crep_inline_helper_probeScript.sml crep_inline_helper_probe.out \
   eoc_p unreach_p "$cake_dir/pancake/crep_inlineScript.sml" "$cake_dir/pancake"
+run_probe crep_inline_eval_probeScript.sml crep_inline_eval_probe.out \
+  src_main_is_call src_var_eq_tgt_var "$cake_dir/pancake/semantics/crepSemScript.sml" \
+  "$cake_dir/pancake/semantics"
 run_probe pan_flat_store_probeScript.sml pan_flat_store_probe.out \
   store_hit stores_blocked "$cake_dir/pancake/semantics/panSemScript.sml"
 run_probe pan_flatten_probeScript.sml pan_flatten_probe.out \
